arm/ConstpropOp.v
@@ -345,6 +345,12 @@ Inductive eval_static_operation_cases: forall (op: operation) (vl: list approx),
   | eval_static_operation_case49:
       forall n1,
       eval_static_operation_cases (Ofloatofint) (I n1 :: nil)
+  | eval_static_operation_case50:
+      forall n1,
+      eval_static_operation_cases (Ointuoffloat) (F n1 :: nil)
+  | eval_static_operation_case53:
+      forall n1,
+      eval_static_operation_cases (Ofloatofintu) (I n1 :: nil)
   | eval_static_operation_case51:
       forall c vl,
       eval_static_operation_cases (Ocmp c) (vl)
@@ -455,6 +461,10 @@ Definition eval_static_operation_match (op: operation) (vl: list approx) :=
       eval_static_operation_case48 n1
   | Ofloatofint, I n1 :: nil =>
       eval_static_operation_case49 n1
+  | Ointuoffloat, F n1 :: nil =>
+      eval_static_operation_case50 n1
+  | Ofloatofintu, I n1 :: nil =>
+      eval_static_operation_case53 n1
   | Ocmp c, vl =>
       eval_static_operation_case51 c vl
   | Oshrximm n, I n1 :: nil =>
@@ -563,6 +573,10 @@ Definition eval_static_operation (op: operation) (vl: list approx) :=
       match Float.intoffloat n1 with Some x => I x | None => Unknown end
   | eval_static_operation_case49 n1 =>
       F(Float.floatofint n1)
+  | eval_static_operation_case50 n1 =>
+      match Float.intuoffloat n1 with Some x => I x | None => Unknown end
+  | eval_static_operation_case53 n1 =>
+      F(Float.floatofintu n1)
   | eval_static_operation_case51 c vl =>
       match eval_static_condition c vl with
       | None => Unknown
